A new way to handle variable renaming proposed and discussed together with David. Proved cover_step.

src/coq/formula.v
@@ -1,4 +1,6 @@
 Require Import List.
+Require Import Classical.
+Require Import Omega.
 
 Module Type Formulas.
   Import ListNotations.
@@ -10,7 +12,11 @@ Module Type Formulas.
   Parameter Var : Type .
   Definition Valuation : Type := Var -> Model .
 
-
+  Parameter var_eq : Var -> Var -> bool .
+  Axiom var_eq_spec_true : forall x y, var_eq x y = true <-> x = y .
+  Axiom var_eq_spec_false : forall x y, var_eq x y = false <-> x <> y .
+  Axiom var_eq_refl : forall x, var_eq x x = true .
+  
   (* FOL *)
   (*
   Parameter FOLFormula : Type .
@@ -64,101 +70,229 @@ Module Type Formulas.
   
   Definition ValidML (phi : MLFormula) : Prop :=
     forall gamma rho, SatML gamma rho phi.
-(*  Definition SatisfiableML (phi : MLFormula) : Prop :=
-    exists gamma rho, SatML gamma rho phi . *)
 
+
+  
   (* Free variables *)
   Parameter getFreeVars : MLFormula -> list Var .
+
+  (* Modify valuation on set *)
+  Definition modify_val_on_var(rho rho' : Valuation) (x : Var) : Valuation :=
+    fun z => if (var_eq x z) then rho' x else rho z .
+
+  Fixpoint modify_val_on_set(rho rho' : Valuation) (X : list Var) : Valuation :=
+    match X with
+      | [] => rho
+      | x :: Xs => modify_val_on_var (modify_val_on_set rho rho' Xs) rho' x
+    end.
   
-  
-  Parameter modify_val_on_set :
-    Valuation -> Valuation -> list Var -> Valuation .
-  
-  Axiom modify_1 :
-    forall x V rho rho',
+  Lemma modify_in :
+    forall V x rho rho',
       In x V -> (modify_val_on_set rho rho' V) x = rho' x.
-  Axiom modify_2 :
+  Admitted.
+    
+  
+  Lemma modify_not_in :
     forall x V rho rho',
       ~ In x V -> (modify_val_on_set rho rho' V) x = rho x.
+  Admitted.
 
-  Axiom modify_Sat1 :
+  
+  Lemma modify_Sat1 :
     forall gamma rho rho' phi V,
       SatML gamma rho' phi ->
-      (forall x, In x (getFreeVars phi) -> In x V) ->
+      incl (getFreeVars phi) V ->
       SatML gamma (modify_val_on_set rho rho' V) phi.
-  Axiom modify_Sat2 :
+  Admitted.
+  
+  Lemma modify_Sat2 :
     forall gamma rho rho' phi V,
       SatML gamma rho phi ->
       (forall x, In x (getFreeVars phi) -> ~ In x V) ->
       SatML gamma (modify_val_on_set rho rho' V) phi.
-
-
-
-    (* renaming *)
+  Admitted.
+  
+  
+  (* renaming stuff *)
   Parameter rename_var : Var -> Var -> MLFormula -> MLFormula.
-  Axiom renamed_removed :
+
+  Axiom new_var_is_free :
     forall x y phi,
-      ~ In x (getFreeVars (rename_var x y phi)).
+      In x (getFreeVars phi) ->
+      In y (getFreeVars (rename_var x y phi)) .
 
-  Axiom rename_sat :
-    forall gamma rho phi x y,
-      SatML gamma rho phi <->
-      SatML gamma rho (rename_var x y phi) .
-
-  Axiom free_rename:
-    forall z x y phi,
+  Axiom new_or_old :
+    forall x y z phi,
       In z (getFreeVars (rename_var x y phi)) ->
-      y = z \/ (x <> z /\ In z (getFreeVars phi)).
+      z = y \/ (z <> y /\ In z (getFreeVars phi)) .
   
   
-  Fixpoint rename_vars (X Y : list Var)
+  Fixpoint rename_var_set (X Y : list Var)
            (phi : MLFormula) : MLFormula :=
     match X, Y with
       | x :: Xs, y :: Ys =>
-        rename_var x y (rename_vars Xs Ys phi)
+        rename_var x y (rename_var_set Xs Ys phi)
+(*        rename_var_set Xs Ys (rename_var x y phi) *)
       | _, _ => phi
     end.
+          
+  
+  Definition rename_val (rho : Valuation) (x y : Var) : Valuation :=
+    fun z => if (var_eq z y) then rho x else rho z .
 
+  Lemma rename_val_not_in :
+    forall z rho x y,
+      z <> x ->  rename_val rho x y z = rho z.
+  Admitted.
+  
+  
+  Lemma rename_sat :
+    forall gamma rho phi x y,
+      SatML gamma rho phi ->
+      ~ In y (getFreeVars phi) ->
+      SatML gamma (rename_val rho x y) (rename_var x y phi) .
+  Admitted.
+
+  Fixpoint rename_val_set (rho : Valuation) (X Y : list Var) : Valuation :=
+    match X, Y with 
+      | x :: Xs, y :: Ys =>
+        rename_val_set (rename_val rho x y) Xs Ys 
+      | _, _ => rho
+    end.
+
+  Lemma rename_sat_set :
+    forall gamma rho phi X Y,
+      SatML gamma rho phi ->
+      (forall y, In y Y -> ~ In y (getFreeVars phi)) ->
+      SatML gamma (rename_val_set rho X Y) (rename_var_set X Y phi).
+  Admitted.
+
+  Lemma rename_val_set_not_in :
+    forall v rho X Y,
+      ~ In v X -> rename_val_set rho X Y v = rho v.
+  Admitted.
+  
+  
+
+  
+(*
   Lemma rename_sat_Set :
     forall gamma rho phi X Y,
       SatML gamma rho phi <->
       SatML gamma rho (rename_vars X Y phi) .
+  Proof.
+    intros gamma rho phi X Y.
+    split; intros H.
+    - induction X.
+      + simpl; trivial.
+      + simpl.
   Admitted.
+*)  
 
   Axiom rename_And :
     forall phi phi' X Y,
-      rename_vars X Y (AndML phi phi') =
-      (AndML (rename_vars X Y phi) (rename_vars X Y phi')).
+      rename_var_set X Y (AndML phi phi') =
+      (AndML (rename_var_set X Y phi) (rename_var_set X Y phi')).
 
   Axiom rename_Not :
     forall phi X Y,
-      rename_vars X Y (NotML phi) =
-      (NotML (rename_vars X Y phi)).
+      rename_var_set X Y (NotML phi) =
+      (NotML (rename_var_set X Y phi)).
 
   
-  Parameter generate_var_not_in_set : Var -> list Var -> Var .
+  Parameter generate_var_not_in_set : list Var -> Var .
   Axiom new_var_not_in_set :
-    forall X x,
-       ~ In (generate_var_not_in_set x X) X.
+    forall X,
+       ~ In (generate_var_not_in_set X) X.
 
-  Fixpoint generate_vars (Vs X : list Var) : list Var :=
-    match Vs with
-      | nil => nil
-      | v :: V =>
-        (generate_var_not_in_set v X) :: generate_vars V X
+  Fixpoint generate_vars (n : nat) (X : list Var) : list Var :=
+    match n with
+      | 0 => nil
+      | S n' => let new_x := generate_var_not_in_set X in
+                new_x :: generate_vars n' (new_x :: X)
     end.
 
-  Axiom rename_exists_sat :
-    forall X Y gamma rho phi,
-      SatML gamma rho (ExistsML X phi) <->
-      SatML gamma rho (ExistsML (generate_vars X Y)
-                                (rename_vars X (generate_vars X Y) phi)).
+  Lemma generate_vars_exact_n :
+    forall n X,
+      n = length (generate_vars n X) .
+  Proof.
+    induction n; simpl; trivial.
+    intros X.
+    apply eq_S.
+    apply IHn.
+  Qed.
 
-  Lemma generated_free :
-    forall Y x phi,
-      In x (getFreeVars (rename_vars (getFreeVars phi) Y phi)) ->
-      In x Y .
-    Admitted.
+    
+
+
+  Lemma replace_all :
+    forall phi Y X y,
+      incl (getFreeVars phi) X ->
+      length X = length Y ->
+      (In y (getFreeVars (rename_var_set X Y phi)) <-> In y Y).
+  Proof.
+  Admitted.      
+    
+
+
+      
+      
+  
+  Lemma generated_vars_not_in_set :
+    forall n X y,
+      In y (generate_vars n X) ->
+      ~ In y X.
+  Proof.
+    induction n; intros.
+    - simpl in H.
+      contradict H.
+    - simpl in H.
+      destruct H as [H | H].
+      + subst y.
+        apply new_var_not_in_set.
+      + apply IHn in H.
+        unfold not in *.
+        intros.
+        apply H.
+        simpl.
+        right.
+        trivial.
+  Qed.
+
+  Lemma generated_vars_not_in :
+    forall n x X Y,
+      In x X ->
+      incl X Y ->
+      ~ In x (generate_vars n Y) .
+  Proof.
+    induction n; intros.
+    - simpl.
+      unfold not.
+      intros.
+      trivial.
+    - simpl.
+      apply and_not_or.
+      split.
+      + assert (H1 : ~ In (generate_var_not_in_set Y) Y).
+        * apply new_var_not_in_set.
+        * unfold not.
+          intros.
+          subst x.
+          unfold incl in H0.
+          apply H0 in H.
+          contradict H1.
+          trivial.
+      + apply IHn with (X := X); trivial.
+        unfold incl.
+        intros a Ha.
+        simpl.
+        right.
+        unfold incl in H0.
+        apply H0 in Ha; trivial.
+  Qed.
+
+
+
   
   (* encoding: ML -> FOL *)
   (* Parameter encoding : MLFormula -> FOLFormula . *)
@@ -179,7 +313,6 @@ Module Type Formulas.
       exists gamma, SatML gamma rho phi.
 
   
-  
   Axiom enc_sat :
     forall gamma rho phi,
       SatML gamma rho (encoding phi) <->
@@ -188,8 +321,7 @@ Module Type Formulas.
 
   Axiom rename_encoding :
     forall phi X Y,
-      rename_vars X Y (encoding phi) =
-      (encoding (rename_vars X Y phi)).
-
+      rename_var_set X Y (encoding phi) =
+      (encoding (rename_var_set X Y phi)).
   
 End Formulas.
